To show how a single ternary constraint such as A+B=CA + B = CA+B=C can be turned into three binary constraints using an auxiliary variable, and how constraints with more than three variables can be treated similarly, and finally how unary constraints can be eliminated by altering the domains of variables, follow these steps:

### Transforming a Ternary Constraint into Binary Constraints

Given the ternary constraint:A+B=CA + B = CA+B=C

1.  Define a new auxiliary variable DDD which takes on values that are pairs (a,b)(a, b)(a,b) where aaa is a value from the domain of AAA and bbb is a value from the domain of BBB. Let DDD be such that:D=(A,B)D = (A, B)D=(A,B)
    
2.  Here, first(D)\\text{first}(D)first(D) and second(D)\\text{second}(D)second(D) represent functions that return the first and second elements of the pair DDD respectively, and sum(D)\\text{sum}(D)sum(D) represents a function that returns the sum of the elements of the pair DDD.
    
    *   **Constraint 1:** The auxiliary variable DDD must represent the pair of values from AAA and BBB:A=first(D)A = \\text{first}(D)A=first(D)
        
    *   **Constraint 2:** Similarly, BBB must match the second element of the pair represented by DDD:B=second(D)B = \\text{second}(D)B=second(D)
        
    *   **Constraint 3:** The sum of AAA and BBB must equal CCC:C=sum(D)C = \\text{sum}(D)C=sum(D)
        

### Example:

Let the domains be:

*   Domain of AAA: {1, 2, 3}
    
*   Domain of BBB: {4, 5, 6}
    
*   Domain of CCC: {5, 6, 7, 8, 9}
    
*   Domain of DDD: {(1, 4), (1, 5), (1, 6), (2, 4), (2, 5), (2, 6), (3, 4), (3, 5), (3, 6)}
    

Then, the binary constraints are:

*   A=first(D)A = \\text{first}(D)A=first(D)
    
*   B=second(D)B = \\text{second}(D)B=second(D)
    
*   C=sum(D)C = \\text{sum}(D)C=sum(D)
    

### Extending to Constraints with More Than Three Variables

For a constraint involving more than three variables, such as:A+B+C=DA + B + C = DA+B+C=D

1.  Define a new auxiliary variable EEE to represent a pair of values (A,B)(A, B)(A,B), and another auxiliary variable FFF to represent the result of the sum of AAA and BBB:E=(A,B)E = (A, B)E=(A,B)F=A+BF = A + BF=A+B
    
2.  **Define Binary Constraints:**
    
    *   A=first(E)A = \\text{first}(E)A=first(E)
        
    *   B=second(E)B = \\text{second}(E)B=second(E)
        
    *   F=sum(E)F = \\text{sum}(E)F=sum(E)
        
    *   F+C=DF + C = DF+C=D
        

Thus, the original constraint A+B+C=DA + B + C = DA+B+C=D is decomposed into a set of binary constraints.

### Eliminating Unary Constraints

Unary constraints can be eliminated by altering the domains of variables.

For example, if we have a unary constraint:A∈{1,2}A \\in \\{1, 2\\}A∈{1,2}

Instead of having this unary constraint, we can directly restrict the domain of AAA to the set {1, 2}.

This demonstrates that any CSP can be transformed into a CSP with only binary constraints by using auxiliary variables and modifying domains.

### Conclusion

By introducing auxiliary variables and altering domains, any Constraint Satisfaction Problem (CSP) can be transformed into a form with only binary constraints. This method systematically decomposes higher-order constraints into simpler binary constraints, making the problem easier to handle using binary CSP solvers.
